feat: change entry definition and add proofs

theories/Semantics.v
@@ -16,11 +16,65 @@ Import MCMonadNotation.
 Definition gal_id :=
   tLambda (BasicAst.nNamed "x"%bs) (tRel 0).
 
-Lemma weaken_ctx : forall Σ' Γ x t ann t',
-  translatesTo remap_env Σ' Γ t ann t' ->
-  translatesTo remap_env Σ' (Γ ++ [x]) t ann t'.
+Lemma lookup_entry_Some : forall Σ_fresh kn kn' br, 
+  lookup_entry Σ_fresh kn = Some (kn, kn', br) ->
+  In kn' (map (snd ∘ fst) Σ_fresh).
 Proof.
-  intros Σ' Γ x t. revert Γ.
+  intros. induction Σ_fresh.
+  - discriminate.
+  - destruct a as [[bd_kn bd_kn'] bd]. 
+    simpl. simpl in H.
+    destruct (bd_kn == kn) eqn:Heq; inversion H; subst.
+    + now left.
+    + apply IHΣ_fresh in H1. now right.
+Qed.
+
+Lemma lookup_fresh_Some : forall Σ_fresh kn kn', 
+  lookup_fresh Σ_fresh kn = Some (kn, kn') ->
+  In kn' (map snd Σ_fresh).
+Proof.
+  intros. induction Σ_fresh.
+  - discriminate.
+  - destruct a as [bd_kn bd_kn']. 
+    simpl. simpl in H. eauto.
+    destruct (bd_kn == kn) eqn:Heq; inversion H; subst.
+    + now left.
+    + apply IHΣ_fresh in H1. now right.
+Qed.
+
+Lemma lookup_init : forall Σ Σ' ann_env kn kn' decl cb,
+  EGlobalEnv.declared_constant (trans_env Σ) kn decl ->
+  decl.(EAst.cst_body) = Some cb ->
+  lookup_fresh (map fst Σ') kn = Some (kn, kn') ->
+  translatesEnv remap_env Σ Σ' ann_env ->
+  exists Σ'' ann_cb cb', translatesTo remap_env Σ'' [] cb ann_cb cb'.
+Proof.
+  intros. induction Σ.
+  - discriminate.
+  - destruct a as [[c_kn c_kn'] c_decl].
+    hnf in H. simpl in H.
+    destruct (kn == c_kn).
+    + destruct c_decl.
+      * inversion H2. subst.
+        destruct entry as [[e_kn e_kn'] [vd b]].
+        destruct c. destruct cst_body; simpl in H9; try eauto.
+        destruct decl. destruct cst_body; try discriminate.
+        inversion H. inversion H0. subst. hnf in ann_decl.
+        exists (map fst Σ'0). exists ann_decl. exists b. 
+        assumption.
+      * inversion H.
+      * inversion H. inversion H2. subst.
+        admit.
+    + inversion H2.
+      * admit.
+      * eapply IHΣ; try eauto.
+Admitted.
+
+Lemma weaken_ctx : forall Σ_fresh Γ x t ann t',
+  translatesTo remap_env Σ_fresh Γ t ann t' ->
+  translatesTo remap_env Σ_fresh (Γ ++ [x]) t ann t'.
+Proof.
+  intros Σ_fresh Γ x t. revert Γ.
   induction t; intros Γ ann t' tlt;
   inversion tlt; subst.
   - constructor.
@@ -41,11 +95,11 @@ Proof.
   - now eapply tlt_const.
 Qed.
 
-Lemma weaken_ctx_many : forall Σ' Γ1 Γ2 t ann t',
-  translatesTo remap_env Σ' Γ1 t ann t' ->
-  translatesTo remap_env Σ' (Γ1 ++ Γ2) t ann t'.
+Lemma weaken_ctx_many : forall Σ_fresh Γ1 Γ2 t ann t',
+  translatesTo remap_env Σ_fresh Γ1 t ann t' ->
+  translatesTo remap_env Σ_fresh (Γ1 ++ Γ2) t ann t'.
 Proof.
-  intros Σ' Γ1 Γ2 t. revert Γ1. induction t;
+  intros Σ_fresh Γ1 Γ2 t. revert Γ1. induction t;
   intros Γ1 ann t' tlt_t; 
   inversion tlt_t; subst.
   - constructor.
@@ -66,12 +120,12 @@ Proof.
   - now eapply tlt_const.
 Qed.
 
-Lemma strengthen_shadowed_ctx : forall Σ' Γ x b ann_b b',
+Lemma strengthen_shadowed_ctx : forall Σ_fresh Γ x b ann_b b',
   In x Γ ->
-  translatesTo remap_env Σ' (Γ ++ [x]) b ann_b b' ->
-  translatesTo remap_env Σ' Γ b ann_b b'.
+  translatesTo remap_env Σ_fresh (Γ ++ [x]) b ann_b b' ->
+  translatesTo remap_env Σ_fresh Γ b ann_b b'.
 Proof.
-  intros Σ' Γ x b. revert Γ. induction b;
+  intros Σ_fresh Γ x b. revert Γ. induction b;
   intros Γ ann_b b' Hin tlt; inversion tlt; subst.
   - constructor.
   - apply tlt_rel.
@@ -127,12 +181,122 @@ Proof.
     exact (f _ _ X).
 Defined.
 
-Lemma csubst_shadowed : forall Σ' Γ x b ann_b b' v ann_v,
-  In x Γ ->
-  translatesTo remap_env Σ' (Γ ++ [x]) b ann_b b' ->
-  translatesTo remap_env Σ' (Γ ++ [x]) (csubst v (List.length Γ) b) (annot_csubst ann_v (List.length Γ) ann_b) b'.
+Fixpoint subst_entries (Σ' : list entry) t {struct Σ'} :=
+  match Σ' with
+  | [] => t
+  | ((_, TermBind (VarDecl kn' ty) b)::Σ'') => 
+      BigStepPIR.subst kn' b (subst_entries Σ'' t)
+  end.
+
+Lemma unfold_app_subst x v' f' a' :
+  BigStepPIR.subst x v' (Apply f' a') = Apply (BigStepPIR.subst x v' f') (BigStepPIR.subst x v' a').
 Proof.
-  intros Σ' Γ x b. revert Γ. induction b; 
+  eauto.
+Qed.
+
+Lemma unfold_app_subst_entries (Σ' : list entry) f' a' :
+  subst_entries Σ' (Apply f' a') = Apply (subst_entries Σ' f') (subst_entries Σ' a').
+Proof.
+  induction Σ'.
+  - eauto.
+  - destruct a as [fr [[] b]].
+    simpl. now rewrite <- unfold_app_subst.
+Qed.
+
+Lemma unfold_let_subst x v' bs t' :
+  BigStepPIR.subst x v' (Let bs t') =
+  Let (@subst_bnr' subst_b x v' bs)
+      (if existsb (eqb x) (bvbs bs)
+        then t'
+        else BigStepPIR.subst x v' t').
+Proof.
+  eauto.
+Qed.
+
+Lemma subst_comm : forall kn kn' v v' b,
+  kn <> kn' ->
+  BigStepPIR.subst kn v (BigStepPIR.subst kn' v' b) = BigStepPIR.subst kn' v' (BigStepPIR.subst kn v b).
+Proof.
+  intros. induction b; try eauto.
+  - admit.
+  - admit.
+  - destruct_str_eq kn' b.
+    + simpl. rewrite Heqb.
+      destruct_str_eq kn b.
+      * subst. contradiction.
+      * simpl. now rewrite Heqb, Heqb0.
+    + simpl. rewrite Heqb.
+      destruct_str_eq kn b.
+      * simpl. now rewrite Heqb, Heqb0.
+      * simpl. now rewrite Heqb, Heqb0, IHb.
+  - simpl. f_equal; eauto.
+Admitted.
+
+Lemma subst_entries_comm : forall (Σ' : list entry) x v b,
+  ~ In x (map (fun '((_, _), TermBind (VarDecl nm _) _) => nm) Σ') ->
+  BigStepPIR.subst x v (subst_entries Σ' b) = subst_entries Σ' (BigStepPIR.subst x v b).
+Proof.
+  intros. induction Σ'.
+  - eauto.
+  - destruct a as [[e_kn e_kn'] [[nm ty] t]].
+    simpl in *. rewrite subst_comm.
+    + now rewrite IHΣ'.
+    + now apply not_in_cons in H as [Hneq HnIn].
+Qed.
+
+Lemma unfold_let_subst_entries Σ' e_kn e_kn' e_ty e_b' bs t' :
+  subst_entries (((e_kn, e_kn'), TermBind (VarDecl e_kn' e_ty) e_b') :: Σ')
+    (Let bs t')
+  =
+  Let
+    (@subst_bnr' subst_b e_kn' e_b' bs)
+    (if existsb (eqb e_kn') (bvbs bs)
+     then t'
+     else (BigStepPIR.subst e_kn' e_b' (subst_entries Σ' t'))).
+Proof.
+  induction Σ'.
+  - eauto.
+  - destruct a as [[a_kn a_kn'] [[nm ty] t]]. simpl in *.
+    admit.
+Admitted. 
+
+Lemma eval_constant_unfolding : forall Σ' kn' b' v' k,
+  (forall e : entry, match e with | ((_, e_kn'), TermBind (VarDecl e_nm _) _) => e_kn' = e_nm end) ->  
+  ~ In kn' (map (fun '((_, _), TermBind (VarDecl nm _) _) => nm) Σ') ->
+  eval (subst_entries Σ' b') v' k ->
+  eval (subst kn' b' (subst_entries Σ' (Var kn'))) v' k.
+Proof.
+  intros. revert b' H1. induction Σ'; intros.
+  - simpl. intros. now rewrite eqb_refl.
+  - destruct a as [[e_kn e_kn'] [[nm ty] t]].
+    rewrite subst_entries_comm; try eauto.
+    simpl. now rewrite eqb_refl.
+Qed.
+
+Lemma eval_value : forall Σ' v' k,
+  eval v' v' k ->
+  exists j, eval (subst_entries Σ' v') v' j.
+Proof.
+  intros Σ' v' k ev. 
+  induction Σ'; eauto.
+  destruct a as [[e_kn e_kn'] [[nm ty] t]].
+  inversion ev; subst.
+  - simpl. rewrite subst_entries_comm; [|admit].
+    simpl. destruct_str_eq nm x.
+    + apply IHΣ'.
+    + admit.
+  - admit.
+  - simpl. now rewrite subst_entries_comm; [|admit].
+  - admit.
+Admitted.
+
+Lemma csubst_shadowed : forall Σ_fresh Γ x b ann_b b' v ann_v,
+  In x Γ ->
+  translatesTo remap_env Σ_fresh (Γ ++ [x]) b ann_b b' ->
+  translatesTo remap_env Σ_fresh (Γ ++ [x]) 
+    (csubst v (List.length Γ) b) (annot_csubst ann_v (List.length Γ) ann_b) b'.
+Proof.
+  intros Σ_fresh Γ x b. revert Γ. induction b; 
   intros Γ ann_b b' v ann_v Hin tlt; inversion tlt.
   - constructor.
   - simpl. unfold find_index_string in H1.
@@ -158,29 +322,16 @@ Proof.
   - now eapply tlt_const.
 Qed.
 
-Lemma lookup_Some : forall Σ' kn kn' br, 
-  lookup_entry Σ' kn = Some (kn, kn', br) ->
-  In kn' (get_binder_names Σ').
-Proof.
-  intros. induction Σ'.
-  - discriminate.
-  - destruct a as [[bd_kn bd_kn'] bd]. 
-    simpl. simpl in H. 
-    destruct (bd_kn == kn) eqn:Heq; inversion H.
-    + now left.
-    + apply IHΣ' in H1. now right.
-Qed.
-
-Lemma csubst_correct : forall Σ' Γ x v b ann_v ann_b v' b',
+Lemma csubst_correct : forall Σ_fresh Γ x v b ann_v ann_b v' b',
   ~ In x Γ ->
-  ~ In x (get_binder_names Σ') ->
-  translatesTo remap_env Σ' [] v ann_v v' ->
-  translatesTo remap_env Σ' (Γ ++ [x]) b ann_b b' ->
-  translatesTo remap_env Σ' Γ (csubst v (List.length Γ) b)
+  ~ In x (get_binder_names Σ_fresh) ->
+  translatesTo remap_env Σ_fresh [] v ann_v v' ->
+  translatesTo remap_env Σ_fresh (Γ ++ [x]) b ann_b b' ->
+  translatesTo remap_env Σ_fresh Γ (csubst v (List.length Γ) b)
   (annot_csubst ann_v (List.length Γ) ann_b)
   (BigStepPIR.subst x v' b').
 Proof.
-  intros Σ' Γ x v b. revert Γ. induction b;
+  intros Σ_fresh Γ x v b. revert Γ. induction b;
   intros Γ ann_v ann_b v' b' HnIn HnIn' tlt_v tlt_b;
   inversion tlt_b; subst.
   - constructor.
@@ -203,9 +354,10 @@ Proof.
     + apply tlt_lambda. 
       * assumption.
       * subst x'. assert (Hin : In x (x::Γ)) by now left.
-        specialize (csubst_shadowed Σ' (x :: Γ) x b ann_b0 b'0 v ann_v Hin H4).
+        specialize (csubst_shadowed Σ_fresh (x :: Γ) x b ann_b0 b'0 v ann_v Hin H4).
         intros. simpl in H.
-        specialize (strengthen_shadowed_ctx Σ' (x :: Γ) x (csubst v (S #|Γ|) b) (annot_csubst ann_v (S #|Γ|) ann_b0) b'0 Hin H) as Hctx'.
+        specialize (strengthen_shadowed_ctx Σ_fresh (x :: Γ) x 
+          (csubst v (S #|Γ|) b) (annot_csubst ann_v (S #|Γ|) ann_b0) b'0 Hin H) as Hctx'.
         apply Hctx'.
     + apply tlt_lambda.
       * assumption.
@@ -216,9 +368,10 @@ Proof.
       * assumption.
       * now apply IHb1. 
       * subst x'. assert (Hin : In x (x::Γ)) by now left.
-        specialize (csubst_shadowed Σ' (x :: Γ) x b2 ann_b0 b'0 v ann_v Hin H6).
+        specialize (csubst_shadowed Σ_fresh (x :: Γ) x b2 ann_b0 b'0 v ann_v Hin H6).
         intros. simpl in H.
-        specialize (strengthen_shadowed_ctx Σ' (x :: Γ) x (csubst v (S #|Γ|) b2) (annot_csubst ann_v (S #|Γ|) ann_b0) b'0 Hin H) as Hctx'.
+        specialize (strengthen_shadowed_ctx Σ_fresh (x :: Γ) x 
+          (csubst v (S #|Γ|) b2) (annot_csubst ann_v (S #|Γ|) ann_b0) b'0 Hin H) as Hctx'.
         apply Hctx'.
     + apply tlt_let.
       * assumption.
@@ -231,28 +384,21 @@ Proof.
     now apply tlt_app.
   - simpl.
     destruct_str_eq x kn'.
-    + apply lookup_Some in H1 as HIn'. subst. contradiction.
+    + apply lookup_fresh_Some in H1 as HIn'. subst. contradiction.
     + econstructor. eauto.
 Qed.
 
-Theorem stlc_correct : forall (Σ : global_env) Σ'
-  t (ann_t : annots box_type t) t' v,
-  (trans_env Σ) e⊢ t ⇓ v ->
-  InSubset Σ [] t ->
-  (* declared entries have been substituted *)
-  (forall kn decl cb ann_cb kn' vdecl cb', 
-    EGlobalEnv.declared_constant (trans_env Σ) kn decl ->
-    decl.(cst_body) = Some cb ->
-    lookup_entry Σ' kn = Some (kn, kn', TermBind vdecl cb') ->
-    translatesTo remap_env Σ' [] cb ann_cb (Var kn')) ->
-  translate_term remap_env Σ' [] t ann_t = Some t' ->
+Theorem stlc_correct : forall t (ann_t : annots box_type t) t' v,
+  (trans_env []) e⊢ t ⇓ v ->
+  InSubset [] [] t ->
+  translate_term remap_env [] [] t ann_t = Some t' ->
   exists ann_v v' k,
-    translatesTo remap_env Σ' [] v ann_v v' /\
+    translatesTo remap_env [] [] v ann_v v' /\
     eval t' v' k.
 Proof with (eauto using eval).
-  intros Σ Σ' t ann_t t' v ev sub_t Hdecl_subst tlt.
+  intros t ann_t t' v ev sub_t tlt.
   apply translate_reflect in tlt; try apply NoDup_nil.
-  apply (val_in_sub Σ [] t v ev) in sub_t as sub_v.
+  apply (val_in_sub [] [] t v ev) in sub_t as sub_v.
   revert t' tlt; induction ev; 
   intros t'' tlt; inversion sub_t.
   - (* □ applied to values, temporary nonsensible case *) admit. 
@@ -263,8 +409,8 @@ Proof with (eauto using eval).
     destruct (IHev1 ann_t1 H1 sub_lambda t1' H5) as [ann_v1 [v1' [k1 [tlt_l ev_l]]]].
     destruct (IHev2 ann_t2 H2 sub_arg t2' H8) as [ann_v2 [v2' [k2 [tlt_v2 ev_v2]]]].
     inversion tlt_l. subst.
-    assert (tlt_sb : translatesTo remap_env Σ' [] (csubst a' 0 b) (annot_csubst ann_v2 0 ann_b) (BigStepPIR.subst x' v2' b')).
-    { eapply csubst_correct; auto. admit. }
+    assert (tlt_sb : translatesTo remap_env [] [] (csubst a' 0 b) (annot_csubst ann_v2 0 ann_b) (BigStepPIR.subst x' v2' b')).
+    { eapply csubst_correct; auto. }
     eapply tlt_in_sub in tlt_sb as sub_sb.
     specialize (IHev3 (annot_csubst ann_v2 0 ann_b) sub_sb sub_v (subst x' v2' b') tlt_sb).
     destruct IHev3 as [ann_v' [v' [k3 [tlt_v ev_v]]]].
@@ -279,8 +425,8 @@ Proof with (eauto using eval).
     inversion tlt. apply inj_pair2 in H8. subst.
     eapply val_in_sub in ev1 as sub_br; eauto.
     destruct (IHev1 ann_br H1 sub_br br' H10) as [ann_v1 [v1' [k1 [tlt_br ev_br]]]].
-    assert (tlt_sb : translatesTo remap_env Σ' [] (csubst b0' 0 b1) (annot_csubst ann_v1 0 ann_b) (BigStepPIR.subst x'0 v1' b')).
-    { eapply csubst_correct; auto. admit. }
+    assert (tlt_sb : translatesTo remap_env [] [] (csubst b0' 0 b1) (annot_csubst ann_v1 0 ann_b) (BigStepPIR.subst x'0 v1' b')).
+    { eapply csubst_correct; auto. }
     eapply tlt_in_sub in tlt_sb as sub_sb.
     specialize (IHev2 (annot_csubst ann_v1 0 ann_b) sub_sb sub_v (subst x'0 v1' b') tlt_sb).
     destruct IHev2 as [ann_v' [v' [k2 [tlt_v ev_v]]]].
@@ -303,16 +449,119 @@ Proof with (eauto using eval).
   - (* fix unguarded *)
     eapply val_in_sub in ev1 as sub_fix; eauto.
     inversion sub_fix.
+  - discriminate.
+  - (* mkApps constr *)
+    eapply val_in_sub in ev1 as sub_apps; eauto.
+    apply mkApps_in_subset in sub_apps as [sub_constr _].
+    inversion sub_constr.
+  - (* atoms applied to values *)
+    subst. induction f16; inversion H1.
+    + inversion ev1. subst. inversion i.
+    + rewrite List.nth_error_nil in H0. discriminate H0.
+    + inversion ev1. subst. inversion i.
+    + (* apply LetIn to value *) admit.
+    + (* apply Apply to value *) admit.
+    + discriminate.
+ (* Atoms *)
+  - subst. inversion tlt. exists ann. exists t''.
+    subst. eexists. split.
+    + apply tlt_tt. 
+    + apply E_Constant. eauto.
+  - (* rel *) subst. inversion i.
+  - (* lambda *) subst. exists ann_t. exists t''. inversion tlt. 
+    subst. eexists. split. 
+    + apply tlt.
+    + apply E_LamAbs. eauto.
+Admitted.
+
+Theorem stlc_globals_correct : forall (Σ : global_env) ann_env Σ'
+  t (ann_t : annots box_type t) t' v,
+  (trans_env Σ) e⊢ t ⇓ v ->
+  EnvInSubset Σ ->
+  translate_env remap_env Σ ann_env = Ok Σ' ->
+  InSubset Σ [] t ->
+  translate_term remap_env (map fst Σ') [] t ann_t = Some t' ->
+  exists ann_v v' k,
+    translatesTo remap_env (map fst Σ') [] v ann_v v' /\
+    eval (subst_entries Σ' t') v' k.
+Proof with (eauto using eval).
+  intros Σ ann_env Σ' t ann_t t' v.
+  intros ev sub_env tle sub_t tlt.
+  apply translate_env_reflect in tle.
+  apply translate_reflect in tlt; try apply NoDup_nil.
+  apply (val_in_sub Σ [] t v ev) in sub_t as sub_v.
+  revert Σ' t' tle tlt; induction ev; 
+  intros Σ' t'' tle tlt; inversion sub_t.
+  - (* □ applied to values, temporary nonsensible case *) admit. 
+  - (* apply *)
+    inversion tlt. subst.
+    eapply val_in_sub in ev1 as sub_lambda; eauto.
+    eapply val_in_sub in ev2 as sub_arg; eauto.
+    destruct (IHev1 ann_t1 H1 sub_lambda Σ' t1' tle H5) as [ann_v1 [v1' [k1 [tlt_l ev_l]]]].
+    destruct (IHev2 ann_t2 H2 sub_arg Σ' t2' tle H8) as [ann_v2 [v2' [k2 [tlt_v2 ev_v2]]]].
+    inversion tlt_l. subst.
+    assert (tlt_sb : translatesTo remap_env (map fst Σ') [] 
+      (csubst a' 0 b) (annot_csubst ann_v2 0 ann_b) (BigStepPIR.subst x' v2' b')).
+    { eapply csubst_correct; auto. simpl. admit. }
+    eapply tlt_in_sub in tlt_sb as sub_sb.
+    specialize (IHev3 (annot_csubst ann_v2 0 ann_b) sub_sb sub_v Σ' (BigStepPIR.subst x' v2' b') tle tlt_sb).
+    destruct IHev3 as [ann_v' [v' [k3 [tlt_v ev_v]]]].
+    exists ann_v'. exists v'. eexists. split.
+    + apply tlt_v.
+    + rewrite unfold_app_subst_entries. eapply E_Apply.
+      * eexists.
+      * apply ev_l.
+      * apply ev_v2.
+      * (* apply ev_v. *) admit.
+  - (* let *)
+    inversion tlt. apply inj_pair2 in H8. subst.
+    eapply val_in_sub in ev1 as sub_br; eauto.
+    destruct (IHev1 ann_br H1 sub_br Σ' br' tle H10) as [ann_v1 [v1' [k1 [tlt_br ev_br]]]].
+    assert (tlt_sb : translatesTo remap_env (map fst Σ') [] 
+      (csubst b0' 0 b1) (annot_csubst ann_v1 0 ann_b) (BigStepPIR.subst x'0 v1' b')).
+    { eapply csubst_correct; auto. admit. }
+    eapply tlt_in_sub in tlt_sb as sub_sb.
+    specialize (IHev2 (annot_csubst ann_v1 0 ann_b) sub_sb sub_v Σ' (subst x'0 v1' b') tle tlt_sb).
+    destruct IHev2 as [ann_v' [v' [k2 [tlt_v ev_v]]]].
+    exists ann_v'. exists v'. eexists. split.
+    + apply tlt_v.
+    + destruct Σ'.
+      * simpl in *. econstructor. econstructor; simpl; eauto. 
+      * destruct e as [[e_kn e_kn'] [[vd ty] e_b']]. assert (e_kn' = vd) by admit. subst.
+        erewrite unfold_let_subst_entries. simpl. admit.
+  - (* mkApps fix *) 
+    eapply val_in_sub in ev1 as sub_apps; eauto.
+    apply mkApps_in_subset in sub_apps as [sub_f _]. 
+    inversion sub_f.
+  - (* fix guarded *) 
+    inversion sub_v.
+    apply mkApps_in_subset in H5 as [sub_fix _].
+    inversion sub_fix.
+  - (* fix unguarded *)
+    eapply val_in_sub in ev1 as sub_fix; eauto.
+    inversion sub_fix.
   - (* const *)
-    evar (ann_b : annots box_type body).
-    eapply IHev.
-    + now assert (decl = decl0 /\ body = cb) by eauto using declared_constant_same.
-    + assumption.
-    + (* requires reasoning over Var that has already been substituted *)
-      assert (decl = decl0 /\ body = cb) by eauto using declared_constant_same.
-      destruct H3. inversion tlt. subst.
-      destruct br as [vd b].
-      eapply Hdecl_subst; try eassumption.
+    assert (decl = decl0 /\ body = cb) by eauto using declared_constant_same.
+    invs H3. clear H0. clear H1.
+    inversion tlt. subst.
+    destruct (lookup_init Σ Σ' ann_env c kn' decl0 cb isdecl e H1 tle) as [Σ'' [ann_cb [cb' tlt_cb]]].
+    (* declarations may be evaluated under a subset of the environment *)
+    assert (Σ'' = (map fst Σ')). { admit. } subst.
+    specialize (IHev ann_cb H2 sub_v Σ' cb' tle tlt_cb).
+    inversion tle; subst.
+    + discriminate.
+    + destruct decl; try inversion H3.
+      destruct entry as [[e_kn e_kn'] [[] e_b']].
+      destruct c0. destruct cst_body; simpl in H3; try eauto.
+      (* the names chosen for each entry is fresh *)
+      simpl. rewrite subst_entries_comm; [|admit].
+      simpl. destruct (b =? kn')%string.
+      * simpl in IHev. 
+          (* need to unfold subst_entries to the declaration *)
+          admit.
+      * (* this binder is not the one substituted for the variable *)
+          admit.
+    + (* type alias case *) admit.
   - (* mkApps constr *)
     eapply val_in_sub in ev1 as sub_apps; eauto.
     apply mkApps_in_subset in sub_apps as [sub_constr _].
@@ -335,12 +584,13 @@ Proof with (eauto using eval).
   - subst. inversion tlt. exists ann. exists t''.
     subst. eexists. split. 
     + apply tlt_tt. 
-    + apply E_Constant. eauto.
+    + admit. (* apply E_Constant. eauto. *)
   - (* rel *) subst. inversion i.
   - (* lambda *) subst. exists ann_t. exists t''. inversion tlt. 
     subst. eexists. split. 
     + apply tlt. 
-    + apply E_LamAbs. eauto.
+    + admit.
+    (* + apply E_LamAbs. eauto. *) 
 Admitted.
 
 (* globals and let binding the environment *)
@@ -355,27 +605,42 @@ Theorem stlc_no_globals : forall
     eval t' v' k.
 Proof with (eauto using eval).
   intros t ann_t t' v ev sub_t tlt.
-  eapply (stlc_correct [] [] t);
-  try discriminate; eauto.
+  eapply (stlc_globals_correct [] tt [] t);
+  try discriminate; eauto. constructor.
 Qed.
 
 Theorem stlc_one_global : forall
   gdecl (ann_env : env_annots box_type [gdecl]) entry t ann_t t' v,
   (trans_env [gdecl]) e⊢ t ⇓ v ->
-  InSubset [gdecl] [] t ->
+  EnvInSubset [gdecl] ->
   translate_env remap_env [gdecl] ann_env = Ok [entry] -> 
-  translate_term remap_env [entry] [] t ann_t = Some t' ->
+  InSubset [gdecl] [] t ->
+  translate_term remap_env [fst entry] [] t ann_t = Some t' ->
   exists ann_v v' k,
-    translatesTo remap_env [entry] [] v ann_v v' /\
-    eval t' v' k.
+    translatesTo remap_env [fst entry] [] v ann_v v' /\
+    eval (subst_entries [entry] t') v' k.
 Proof with (eauto using eval).
-  intros gdecl ann_decl entry t ann_t t' v ev sub_t tlt_env tlt.
-  eapply (stlc_correct); try eauto.
-  (* establish invariant *) admit.
+  intros gdecl ann_env entry t ann_t t' v ev sub_env tle sub_t tlt.
+  apply translate_reflect in tlt; try apply NoDup_nil.
+  revert t' tlt; induction ev; 
+  intros t'' tlt; inversion sub_t.
+  - admit.
+  - destruct entry as [[e_kn e_kn'] [[vd ty'] b']]. subst.
+    admit.
+  - admit.
+  - subst. eapply val_in_sub, mkApps_in_subset in ev1 as [not_sub_fix _]; eauto.
+    inversion not_sub_fix.
+  - subst. eapply val_in_sub, mkApps_in_subset in ev1 as [not_sub_fix _]; eauto.
+    inversion not_sub_fix.
+  - admit.
+  - assert (decl = decl0 /\ body = cb) by eauto using declared_constant_same.
+    inversion tlt. invs H3. clear H0. clear H1.
+    destruct entry as [[e_kn e_kn'] [[vd ty] e_b']].
+    simpl. simpl in H6. admit.
 Admitted.
 
 Lemma let_binding_env_correct : forall Σ' t ann_t t' t'',
-  translate_term remap_env (List.rev Σ') [] t ann_t = Some t'' ->
+  translate_term remap_env (List.rev (map fst Σ')) [] t ann_t = Some t'' ->
   translate_term remap_env [] [] t ann_t = Some (bind_pir_env Σ' t').
 Proof.
   intros. unfold bind_pir_env in *.
@@ -398,7 +663,7 @@ Theorem stlc_program_correct : forall eΣ env_ann init cb t v t',
   EGlobalEnv.declared_constant (trans_env eΣ) init cb ->
   cb.(cst_body) = Some t ->
   (trans_env eΣ) e⊢ t ⇓ v ->
-  all_in_subset eΣ ->
+  EnvInSubset eΣ ->
   translate_typed_eprogram remap_env ((eΣ; env_ann), init) = Ok t' ->
   exists ann_v v' k,
     translatesTo remap_env [] [] v ann_v v' /\
@@ -406,10 +671,10 @@ Theorem stlc_program_correct : forall eΣ env_ann init cb t v t',
 Proof.
   intros.
   unfold translate_typed_eprogram in H3.
-  destruct (translate_env remap_env eΣ env_ann) as [Σ'|] eqn:tl_env; try discriminate.
-  apply translate_env_reflect in tl_env.
-  destruct (lookup_entry Σ' init) as [entry|] eqn:Hl; try discriminate.
-  induction tl_env; subst.
+  destruct (translate_env remap_env eΣ env_ann) as [Σ_fresh|] eqn:tle; try discriminate.
+  apply translate_env_reflect in tle.
+  destruct (lookup_entry Σ_fresh init) as [entry|] eqn:Hl; try discriminate.
+  induction tle; subst.
   - inversion Hl.
   - (* valid global *)
     destruct decl; try inversion H4.
