theories/Translation.v
@@ -41,10 +41,13 @@ Section translate.
 
 Context (TT : env PIR.ty).
 
-Definition entry := kername * binderName * binding.
+Definition fresh_pair := kername * binderName. 
+Definition fresh_map := list (kername * binderName).
 
-Definition get_binder_names (Σ' : list entry) : list string :=
-  map (fun '(_, kn', _) => kn') Σ'.
+Definition entry := fresh_pair * binding.
+
+Definition get_binder_names (Σ' : list fresh_pair) : list string :=
+  map snd Σ'.
 
 Definition gen_fresh_name na Σ' Γ :=
   match na with
@@ -69,8 +72,8 @@ Definition translate_ty : box_type -> option PIR.ty :=
   end.
 
 (* Interface so it is easy to add qualified part or change casing later *)
-Definition gen_fresh_binder_name (kn : kername) (bs : list string) :=
-  gen_fresh (kn.2) bs.
+Definition gen_fresh_binder_name (kn : kername) (Σ_fresh : fresh_map) :=
+  gen_fresh (kn.2) (map snd Σ_fresh).
 
 Definition lookup_constant_body (env : ExAst.global_env) kn : option EAst.term :=
   cst <- lookup_constant env kn ;;
@@ -79,8 +82,11 @@ Definition lookup_constant_body (env : ExAst.global_env) kn : option EAst.term :
 Definition lookup_entry (Σ' : list entry) (nm : kername) : option entry :=
   find (fun '(kn, _, _) => eq_kername kn nm) Σ'.
 
+Definition lookup_fresh (Σ_fresh : list fresh_pair) (nm : kername) : option fresh_pair :=
+  find (fun '(kn, _) => eq_kername kn nm) Σ_fresh.
+
 Fixpoint translate_term
-         (Σ' : list entry) (Γ : list string)
+         (Σ_fresh : list fresh_pair) (Γ : list string)
          (t : term) {struct t} : annots box_type t -> option PIR.term :=
   match t return annots box_type t -> option PIR.term with
   | tBox => fun b_ty => Some (PIR.Constant (ValueOf DefaultUniUnit tt)) (* temporary constant *)
@@ -92,35 +98,35 @@ Fixpoint translate_term
   | tLambda x b => fun '(ty, ann_b) =>
     match ty with
     | TArr br_ty _ =>
-      let x' := gen_fresh_name x Σ' Γ in
+      let x' := gen_fresh_name x Σ_fresh Γ in
       br_ty' <- translate_ty br_ty ;;
-      b' <- translate_term Σ' (x' :: Γ) b ann_b ;;
+      b' <- translate_term Σ_fresh (x' :: Γ) b ann_b ;;
       Some (LamAbs x' br_ty' b')
     | _ => None
     end
   | tLetIn x br b => fun '(ty, (ann_br, ann_b)) =>
     match ty with
     | TArr br_ty _ =>
-      let x' := gen_fresh_name x Σ' Γ in
+      let x' := gen_fresh_name x Σ_fresh Γ in
       br_ty' <- translate_ty br_ty ;; 
-      br' <- translate_term Σ' Γ br ann_br ;;
-      b' <- translate_term Σ' (x' :: Γ) b ann_b ;;
+      br' <- translate_term Σ_fresh Γ br ann_br ;;
+      b' <- translate_term Σ_fresh (x' :: Γ) b ann_b ;;
       Some (Let [TermBind (VarDecl x' br_ty') br'] b')
     | _ => None
     end
   | tApp f a => fun '(_, (ann_f, ann_a)) =>
-    f' <- translate_term Σ' Γ f ann_f ;;
-    a' <- translate_term Σ' Γ a ann_a ;;
+    f' <- translate_term Σ_fresh Γ f ann_f ;;
+    a' <- translate_term Σ_fresh Γ a ann_a ;;
     Some (Apply f' a')
   | tConst kn => fun bt =>
-    match lookup_entry Σ' kn with
-    | Some (_, kn', _)=> Some (Var kn')
+    match lookup_fresh Σ_fresh kn with
+    | Some (_, kn') => Some (Var kn')
     | None => None end
   | _ => fun _ => None
   end.
 
 Definition translate_constant
-           (Σ' : list entry)
+           (Σ_fresh : fresh_map)
            (cst : constant_body)
            (kn : kername)
            (ann_c : constant_body_annots box_type cst) : option entry.
@@ -128,8 +134,8 @@ Proof.
   destruct cst as [[params ty] body].
   destruct body as [t|]; [|exact None]. (* no axioms allowed *)
   destruct (translate_ty ty) as [ty'|]; [|exact None].
-  destruct (translate_term Σ' [] t ann_c) as [t'|]; [|exact None].
-  pose (kn' := gen_fresh_binder_name kn (map (fun '(_, nm, _) => nm) Σ')).
+  destruct (translate_term Σ_fresh [] t ann_c) as [t'|]; [|exact None].
+  pose (kn' := gen_fresh_binder_name kn Σ_fresh).
   exact (Some (kn, kn', TermBind (VarDecl kn' ty') t')).
 Defined.
 
@@ -143,7 +149,7 @@ Fixpoint translate_env (eΣ : global_env) : env_annots box_type eΣ -> result (l
     | Ok Σ' =>
       match decl, ann_d with
       | ConstantDecl cst, ann_c =>
-        match translate_constant Σ' cst kn ann_c with
+        match translate_constant (map fst Σ') cst kn ann_c with
         | Some entry => Ok (entry :: Σ')
         | None => Err ("Failed to translate constant " ++ kn_to_s kn)
         end
@@ -187,61 +193,6 @@ Inductive translatesTypeTo : box_type -> PIR.ty -> Prop :=
       lookup TT (string_of_kername ind.(inductive_mind)) = Some ty' ->
       translatesTypeTo (TInd ind) ty'.
 
-Inductive translatesTo (Σ' : list entry) (Γ : list string) : forall (t : term),
-  annots box_type t -> PIR.term -> Prop :=
-  | tlt_tt : forall ann, translatesTo Σ' Γ tBox ann (Constant (ValueOf DefaultUniUnit tt))
-  | tlt_rel : forall n x ann,
-      find_index_string Γ x = Some n ->
-      translatesTo Σ' Γ (tRel n) ann (Var x)
-  | tlt_lambda : forall x x' arg_ty res_ty b ann_b arg_ty' b',
-      translatesTypeTo arg_ty arg_ty' ->
-      translatesTo Σ' (x' :: Γ) b ann_b b' ->
-      translatesTo Σ' Γ (tLambda x b) (TArr arg_ty res_ty, ann_b) (LamAbs x' arg_ty' b')
-  | tlt_let : forall x x' br_ty b_ty br b ann_br ann_b br_ty' br' b',
-      translatesTypeTo br_ty br_ty' ->
-      translatesTo Σ' Γ br ann_br br' ->
-      translatesTo Σ' (x' :: Γ) b ann_b b' ->
-      translatesTo Σ' Γ (tLetIn x br b) (TArr br_ty b_ty, (ann_br, ann_b)) (Let [(TermBind (VarDecl x' br_ty') br')] b')
-  | tlt_app : forall t1 t2 ann_t1 ann_t2 ty t1' t2',
-      translatesTo Σ' Γ t1 ann_t1 t1' ->
-      translatesTo Σ' Γ t2 ann_t2 t2' ->
-      translatesTo Σ' Γ (tApp t1 t2) (ty, (ann_t1, ann_t2)) (PIR.Apply t1' t2')
-  | tlt_const : forall kn kn' br ann,
-      lookup_entry Σ' kn = Some (kn, kn', br) ->
-      translatesTo Σ' Γ (tConst kn) ann (Var kn').
-
-Definition translatesConstant (Σ' : list entry) 
-           (cb : constant_body) (ann_cb : constant_body_annots box_type cb)
-           (cb' : entry) : Prop.
-Proof.
-  destruct cb as [args cst_body].
-  destruct cb' as [[e_kn e_kn'] [v t']].
-  - destruct cst_body.
-    + exact (translatesTo Σ' [] t ann_cb t').
-    + exact False.
-Defined.
-
-Definition translatesDecl (Σ' : list entry) 
-           (decl : global_decl) (ann_decl : global_decl_annots box_type decl)
-           (entry : entry) : Prop.
-Proof.
-  destruct decl.
-  - simpl in ann_decl.
-    exact (translatesConstant Σ' c ann_decl entry).
-  - exact False.
-  - exact False.
-Defined.
-
-Inductive translatesEnv : forall (Σ : global_env) (Σ' : list entry), env_annots box_type Σ -> Prop :=
-  | tlte_empty : forall ann_env, translatesEnv [] [] ann_env
-  | tlte_const : forall Σ Σ' kn deps decl ann_decl entry (ann_env : env_annots box_type Σ),
-      translatesDecl Σ' decl ann_decl entry ->
-      translatesEnv (((kn, deps), decl) :: Σ) (entry :: Σ') (ann_decl, ann_env)
-  | tlte_remap : forall Σ Σ' kn deps ind ann_ind ann_env,
-      find (fun nm : kername => kn == nm) pir_ignore_default = Some kn ->
-      translatesEnv Σ Σ' ann_env ->
-      translatesEnv (((kn, deps), InductiveDecl ind) :: Σ) Σ' (ann_ind, ann_env).
-
 Theorem translate_type_reflect : forall ty ty',
   translate_ty ty = Some ty' -> translatesTypeTo ty ty'.
 Proof.
@@ -257,11 +208,34 @@ Proof.
     + now apply tlty_ind.
 Qed.
 
-Theorem translate_reflect : forall Σ' Γ t t' (ann : annots box_type t),
+Inductive translatesTo (Σ_fresh : fresh_map) (Γ : list string) : forall (t : term),
+  annots box_type t -> PIR.term -> Prop :=
+  | tlt_tt : forall ann, translatesTo Σ_fresh Γ tBox ann (Constant (ValueOf DefaultUniUnit tt))
+  | tlt_rel : forall n x ann,
+      find_index_string Γ x = Some n ->
+      translatesTo Σ_fresh Γ (tRel n) ann (Var x)
+  | tlt_lambda : forall x x' arg_ty res_ty b ann_b arg_ty' b',
+      translatesTypeTo arg_ty arg_ty' ->
+      translatesTo Σ_fresh (x' :: Γ) b ann_b b' ->
+      translatesTo Σ_fresh Γ (tLambda x b) (TArr arg_ty res_ty, ann_b) (LamAbs x' arg_ty' b')
+  | tlt_let : forall x x' br_ty b_ty br b ann_br ann_b br_ty' br' b',
+      translatesTypeTo br_ty br_ty' ->
+      translatesTo Σ_fresh Γ br ann_br br' ->
+      translatesTo Σ_fresh (x' :: Γ) b ann_b b' ->
+      translatesTo Σ_fresh Γ (tLetIn x br b) (TArr br_ty b_ty, (ann_br, ann_b)) (Let [(TermBind (VarDecl x' br_ty') br')] b')
+  | tlt_app : forall t1 t2 ann_t1 ann_t2 ty t1' t2',
+      translatesTo Σ_fresh Γ t1 ann_t1 t1' ->
+      translatesTo Σ_fresh Γ t2 ann_t2 t2' ->
+      translatesTo Σ_fresh Γ (tApp t1 t2) (ty, (ann_t1, ann_t2)) (PIR.Apply t1' t2')
+  | tlt_const : forall kn kn' ann,
+      lookup_fresh Σ_fresh kn = Some (kn, kn') ->
+      translatesTo Σ_fresh Γ (tConst kn) ann (Var kn').
+
+Theorem translate_reflect : forall (Σ_fresh : fresh_map) Γ t t' (ann : annots box_type t),
   NoDup Γ ->
-  translate_term Σ' Γ t ann = Some t' -> translatesTo Σ' Γ t ann t'.
+  translate_term Σ_fresh Γ t ann = Some t' -> translatesTo Σ_fresh Γ t ann t'.
 Proof.
-  intros Σ' Γ t. revert Γ. induction t; try discriminate; 
+  intros Σ_fresh Γ t. revert Γ. induction t; try discriminate; 
   intros Γ t' ann nodup tl_t; inversion tl_t as [Ht].
   - apply tlt_tt.
   - destruct (nth_error Γ n) eqn:El; [|discriminate].
@@ -269,8 +243,8 @@ Proof.
     now apply nth_error_to_find_index in El. 
   - destruct ann as [[] ann_b]; try discriminate.
     destruct (translate_ty dom) as [br_ty'|] eqn:tl_ty; [|discriminate].
-    destruct (translate_term Σ' (gen_fresh_name na Σ' Γ :: Γ) t ann_b) as [b'|] eqn:tl_b; 
-    [|discriminate]. inversion Ht as [Ht']. set (na' := gen_fresh_name na Σ' Γ). 
+    destruct (translate_term Σ_fresh (gen_fresh_name na Σ_fresh Γ :: Γ) t ann_b) as [b'|] eqn:tl_b; 
+    [|discriminate]. inversion Ht as [Ht']. set (na' := gen_fresh_name na Σ_fresh Γ). 
     assert (nodup' : NoDup (na' :: Γ)).
     apply NoDup_cons; try assumption.
     apply gen_fresh_name_fresh.
@@ -279,9 +253,9 @@ Proof.
     now apply tlt_lambda.
   - destruct ann as [[] [ann_br ann_b]]; try discriminate.
     destruct (translate_ty dom) as [br_ty'|] eqn:tl_ty; [|discriminate].
-    destruct (translate_term Σ' Γ t1 ann_br) as [br'|] eqn:tl_br; [|discriminate].
-    destruct (translate_term Σ' (gen_fresh_name na Σ' Γ :: Γ) t2 ann_b) as [b'|] eqn:tl_b; 
-    [|discriminate]. inversion Ht as [Ht']. set (na' := gen_fresh_name na Σ' Γ).
+    destruct (translate_term Σ_fresh Γ t1 ann_br) as [br'|] eqn:tl_br; [|discriminate].
+    destruct (translate_term Σ_fresh (gen_fresh_name na Σ_fresh Γ :: Γ) t2 ann_b) as [b'|] eqn:tl_b; 
+    [|discriminate]. inversion Ht as [Ht']. set (na' := gen_fresh_name na Σ_fresh Γ).
     assert (nodup' : NoDup (na' :: Γ)).
     apply NoDup_cons; try assumption. 
     apply gen_fresh_name_fresh.
@@ -290,23 +264,56 @@ Proof.
     apply (translate_type_reflect dom br_ty') in tl_ty.
     now apply tlt_let.
   - destruct ann as [ty [ann_t1 ann_t2]].
-    destruct (translate_term Σ' Γ t1 ann_t1) as [t1'|] eqn:tl_t1; [|discriminate].
-    destruct (translate_term Σ' Γ t2 ann_t2) as [t2'|] eqn:tl_t2; [|discriminate].
+    destruct (translate_term Σ_fresh Γ t1 ann_t1) as [t1'|] eqn:tl_t1; [|discriminate].
+    destruct (translate_term Σ_fresh Γ t2 ann_t2) as [t2'|] eqn:tl_t2; [|discriminate].
     inversion Ht as [Ht'].
     specialize (IHt1 Γ t1' ann_t1 nodup tl_t1).
     specialize (IHt2 Γ t2' ann_t2 nodup tl_t2).
     now apply tlt_app.
-  - destruct (lookup_entry Σ' k) as [[[kn kn'] br]|] eqn:El; [|discriminate].
-    inversion Ht as [Ht']. apply find_some in El as Hl.
+  - destruct (lookup_fresh Σ_fresh k) as [[kn kn']|] eqn:El; [|discriminate].
+    invs Ht. apply find_some in El as Hl.
     destruct Hl as [Hin Heq]. apply ReflectEq.eqb_eq in Heq. subst.
     now eapply tlt_const.
 Qed.
+
+Definition translatesConstant (Σ_fresh : fresh_map) 
+           (cb : constant_body) (ann_cb : constant_body_annots box_type cb)
+           (cb' : entry) : Prop.
+Proof.
+  destruct cb as [args cst_body].
+  destruct cb' as [[e_kn e_kn'] [v t']].
+  - destruct cst_body.
+    + exact (translatesTo Σ_fresh [] t ann_cb t').
+    + exact False.
+Defined.
+
+Definition translatesDecl (Σ_fresh : fresh_map) 
+           (decl : global_decl) (ann_decl : global_decl_annots box_type decl)
+           (entry : entry) : Prop.
+Proof.
+  destruct decl.
+  - simpl in ann_decl.
+    exact (translatesConstant Σ_fresh c ann_decl entry).
+  - exact False.
+  - exact False.
+Defined.
+
+Inductive translatesEnv : forall (Σ : global_env) (Σ' : list entry), env_annots box_type Σ -> Prop :=
+  | tlte_empty : forall ann_env, translatesEnv [] [] ann_env
+  | tlte_const : forall Σ Σ' kn deps decl ann_decl entry ann_env,
+      translatesDecl (map fst Σ') decl ann_decl entry ->
+      translatesEnv Σ Σ' ann_env ->
+      translatesEnv (((kn, deps), decl) :: Σ) (entry :: Σ') (ann_decl, ann_env)
+  | tlte_remap : forall Σ Σ' kn deps ind ann_ind ann_env,
+      find (fun nm : kername => kn == nm) pir_ignore_default = Some kn ->
+      translatesEnv Σ Σ' ann_env ->
+      translatesEnv (((kn, deps), InductiveDecl ind) :: Σ) Σ' (ann_ind, ann_env).
 
 Theorem translate_env_reflect : forall Σ Σ' ann_env,
   translate_env Σ ann_env = Ok Σ' -> translatesEnv Σ Σ' ann_env.
 Proof.
   intros Σ Σ' ann_env tl_env.
-  induction Σ.
+  revert Σ' tl_env; induction Σ; intros.
   - inversion tl_env. 
     apply tlte_empty.
   - destruct ann_env as [ann_decl ann_env'].
@@ -314,17 +321,18 @@ Proof.
     simpl in tl_env.
     destruct (translate_env Σ ann_env') as [Σ''|err] eqn:tl_env'; try discriminate.
     destruct decl.
-    + destruct (translate_constant Σ'' c kn ann_decl) eqn:tl_constant; try discriminate.
+    + destruct (translate_constant (map fst Σ'') c kn ann_decl) eqn:tl_constant; try discriminate.
       inversion tl_env. subst.
-      econstructor. simpl. 
+      econstructor. simpl.
       destruct c as [[nm ty] [t|]]; try discriminate.
-      { simpl in tl_constant.
+      * simpl in tl_constant.
         destruct (translate_ty ty) eqn:tl_ty; try discriminate.
-        destruct (translate_term Σ'' [] t ann_decl) eqn:tl_t; try discriminate.
+        destruct (translate_term (map fst Σ'') [] t ann_decl) eqn:tl_t; try discriminate.
         apply translate_reflect in tl_t; [|apply NoDup_nil].
         destruct e as [[e_kn e_kn'] [v t']]. simpl.
         inversion tl_constant. subst t1.
-        assumption. }
+        assumption.
+      * eauto.
     + destruct (find (fun nm : kername => kn == nm) pir_ignore_default) eqn:Hremap; try discriminate.
       inversion tl_env. subst.
       apply find_some in Hremap as Heq. 
@@ -338,25 +346,24 @@ End translate.
 Definition translate_unsafe Γ (t : term) (ann : annots box_type t) := 
   with_default (PIR.Error (PIR.UNDEFINED "TranslationFailed")) (translate_term remap_env [] Γ t ann).
 
-(* Lambda Box T is the combination of an EAst term with a dependent tree of its types *)
+(* Lambda Box T is the combination of an EAst term with a dependent tree containing its box types *)
 Definition identity_EAst : term :=
-  tLambda (nNamed "x") 
-    (tRel 0).
+  tLambda (nNamed "x") (tRel 0).
 
 Definition Z_ind := TInd (mkInd <%% Z %%> 0).
 Definition ann_id :=
   (TArr Z_ind Z_ind, Z_ind).
 
+(* Eval cbv in (translate_unsafe [] identity_EAst ann_id). *)
+
 Definition id_twice := tLambda (nNamed "y") (tApp (tConst <%% identity_EAst %%>) (tRel 0)).
 Definition ann_twice := (TArr Z_ind Z_ind, (Z_ind, (TArr Z_ind Z_ind, Z_ind))).
 
-Definition c_id : constant_body := Build_constant_body ([], ann_id.1) (Some identity_EAst).
-Definition decl_id := (<%% identity_EAst %%>, false, Ex.ConstantDecl c_id).
+Definition cst_id : constant_body := Build_constant_body ([], ann_id.1) (Some identity_EAst).
+Definition decl_id := (<%% identity_EAst %%>, false, Ex.ConstantDecl cst_id).
 
-Definition c_twice := Build_constant_body ([], ann_twice.1) (Some id_twice).
-Definition decl_twice := (<%% id_twice %%>, false, Ex.ConstantDecl c_twice).
+Definition cst_twice := Build_constant_body ([], ann_twice.1) (Some id_twice).
+Definition decl_twice := (<%% id_twice %%>, false, Ex.ConstantDecl cst_twice).
 
-(* Eval cbv in (translate_unsafe [] identity_EAst ann_id). *)
-
-Definition example : (∑ env, env_annots box_type env) := ([decl_twice; decl_id]; (ann_twice, (ann_id, tt))).
-(* Eval vm_compute in translate_typed_eprogram remap_env (example, <%% id_twice %%>). *)
+Definition program_example : (∑ env, env_annots box_type env) := ([decl_twice; decl_id]; (ann_twice, (ann_id, tt))).
+(* Eval vm_compute in translate_typed_eprogram remap_env (program_example, <%% id_twice %%>). *)
